riscv ainvs: strengthen valid_uses for C sync; prove it consistent
C now has a user_vtop different from pptr_base, so valid_uses needed updating,
and since the intervals don't fully join up any more, also strengthening of the
user and kernel window properties.

To make sure this is all still consistent, there is now an example state in
ArchKernelInit_AI that is shown to satisfy these conditions.

proof/invariant-abstract/RISCV64/ArchInvariants_AI.thy
@@ -650,11 +650,12 @@ definition valid_uses_2 :: "(obj_ref \<Rightarrow> riscvvspace_region_use) \<Rig
      \<forall>p. (\<not>canonical_address p \<longrightarrow> uses p = RISCVVSpaceInvalidRegion)
           \<and> (p \<in> {pptr_base ..< kernel_base}
              \<longrightarrow> uses p \<in> {RISCVVSpaceKernelWindow, RISCVVSpaceInvalidRegion})
+          \<and> (uses p = RISCVVSpaceKernelWindow \<longrightarrow> p \<in> {pptr_base ..< kernel_base})
           \<comment> \<open>Ordinarily there would be another region on top of the RISCVVSpaceKernelELFWindow
              for devices, but Spike does not have any.\<close>
           \<and> (kernel_base \<le> p \<longrightarrow> uses p \<in> {RISCVVSpaceKernelELFWindow, RISCVVSpaceInvalidRegion})
-          \<comment> \<open>We allow all unreserved canonical virtual addresses as the user window:\<close>
-          \<and> (p < user_vtop \<longrightarrow> canonical_address p \<longrightarrow> uses p = RISCVVSpaceUserRegion)
+          \<comment> \<open>We allow precisely all canonical virtual addresses below user_vtop as the user window:\<close>
+          \<and> (p \<le> user_vtop \<and> canonical_address p \<longleftrightarrow> uses p = RISCVVSpaceUserRegion)
       \<comment> \<open>We want the kernel window to be non-empty, and to contain at least @{const pptr_base}\<close>
       \<and> uses pptr_base = RISCVVSpaceKernelWindow"
 
@@ -1300,6 +1301,29 @@ lemma valid_arch_tcb_typ_at:
   "\<lbrakk> valid_arch_tcb t s; \<And>T p. typ_at T p s \<Longrightarrow> typ_at T p s' \<rbrakk> \<Longrightarrow> valid_arch_tcb t s'"
   by (simp add: valid_arch_tcb_def)
 
+lemma user_vtop_ge0[intro!,simp]:
+  "0 < user_vtop"
+  by (simp add: user_vtop_def pptrUserTop_def pptrBase_def canonical_bit_def mask_def)
+
+lemma user_vtop_pptr_base[intro!,simp]:
+  "user_vtop < pptr_base"
+  by (simp add: user_vtop_def pptrUserTop_def pptr_base_def pptrBase_def canonical_bit_def mask_def)
+
+lemma pptr_base_kernel_base:
+  "pptr_base < kernel_base"
+  by (simp add: pptr_base_def pptrBase_def canonical_bit_def kernel_base_def)
+
+lemma above_pptr_base_canonical:
+  "pptr_base \<le> p \<Longrightarrow> canonical_address p"
+  by (simp add: canonical_address_range pptr_base_def pptrBase_def NOT_mask)
+
+lemma below_user_vtop_canonical:
+  "p \<le> user_vtop \<Longrightarrow> canonical_address p"
+  apply (simp add: user_vtop_def pptrUserTop_def canonical_address_range)
+  apply (rule disjI1, drule order_trans, rule word_and_le2)
+  apply simp
+  done
+
 lemmas window_defs =
   kernel_window_def not_kernel_window_def kernel_elf_window_def kernel_regions_def
   kernel_device_window_def user_region_def
@@ -1307,7 +1331,7 @@ lemmas window_defs =
 lemma valid_uses_kernel_window:
   "\<lbrakk> valid_uses s; p \<in> kernel_window s \<rbrakk> \<Longrightarrow> p \<in> {pptr_base ..< kernel_base} \<and> canonical_address p"
   unfolding valid_uses_def window_defs
-  by (erule_tac x=p in allE) (auto simp: user_vtop_def pptrUserTop_def pptr_base_def)
+  by (erule_tac x=p in allE) auto
 
 lemma valid_uses_user_region:
   "\<lbrakk> valid_uses s; p \<in> user_region s \<rbrakk> \<Longrightarrow> p < pptr_base"
@@ -1618,13 +1642,9 @@ lemma canonical_address_0[intro!,simp]:
   "canonical_address 0"
   by (simp add: canonical_address_def canonical_address_of_def)
 
-lemma user_vtop_ge0[intro!,simp]:
-  "0 < user_vtop"
-  by (simp add: user_vtop_def pptrUserTop_def pptrBase_def canonical_bit_def)
-
 lemma user_region0[intro!,simp]:
   "valid_uses s \<Longrightarrow> 0 \<in> user_region s"
-  by (simp add: valid_uses_def user_region_def)
+  by (force simp: valid_uses_def user_region_def)
 
 lemma pool_for_asid_valid_vspace_objs:
   "\<lbrakk> pool_for_asid asid s = Some p;
@@ -1841,10 +1861,6 @@ lemma valid_vspace_objsD:
    valid_vspace_obj level ao s"
   by (simp add: valid_vspace_objs_def)
 
-lemma user_vtop[simp]:
-  "user_vtop = pptr_base"
-  by (simp add: user_vtop_def pptrUserTop_def pptr_base_def)
-
 lemma pptr_base_mask:
   "pptr_base = ~~mask canonical_bit"
   by (simp add: pptr_base_def pptrBase_def mul_not_mask_eq_neg_shiftl flip: minus_one_shift)
@@ -1854,9 +1870,11 @@ lemma pptr_base_nth[simp]:
   by (simp add: pptr_base_mask neg_mask_bang word_bits_def)
 
 lemma valid_uses_user_region_eq:
-  "valid_uses s \<Longrightarrow> (p \<in> user_region s) = (p < pptr_base \<and> canonical_address p)"
+  "valid_uses s \<Longrightarrow> (p \<in> user_region s) = (p \<le> user_vtop)"
+  using below_user_vtop_canonical[of p]
   unfolding valid_uses_def user_region_def
-  by (erule_tac x=p in allE) (auto simp: not_le)
+  apply clarsimp
+  by (erule_tac x=p in allE) auto
 
 lemma pt_bits_left_bound:
   "pt_bits_left level \<le> canonical_bit + 1"
@@ -1884,22 +1902,26 @@ lemma pt_bits_left_le_max_pt_level:
 lemma canonical_vref_for_levelI:
   "\<lbrakk> canonical_address vref; vref < pptr_base \<rbrakk> \<Longrightarrow> canonical_address (vref_for_level vref level)"
   using pt_bits_left_bound[of level]
-  apply (simp add: canonical_address_def canonical_address_of_def vref_for_level_def pptr_base_mask bit_simps)
+  apply (simp add: canonical_address_def canonical_address_of_def vref_for_level_def pptr_base_mask
+                   bit_simps)
   apply word_bitwise
   by (clarsimp simp: canonical_bit_def word_size not_less)
 
 
+lemma vref_for_level_le:
+  "vref_for_level vref level \<le> vref"
+  by (simp add: vref_for_level_def word_and_le2)
+
 lemma vref_for_level_user_region:
   "\<lbrakk> vref \<in> user_region s; valid_uses s \<rbrakk> \<Longrightarrow> vref_for_level vref level \<in> user_region s"
-  by (clarsimp simp: valid_uses_user_region_eq vref_for_level_pptr_baseI canonical_vref_for_levelI)
+  using vref_for_level_le[of vref level]
+  by (force simp: valid_uses_user_region_eq vref_for_level_pptr_baseI canonical_vref_for_levelI)
 
 lemma aligned_canonical_max_is_0:
   "\<lbrakk> canonical_address p; is_aligned p (pt_bits_left (max_pt_level + 1)) \<rbrakk> \<Longrightarrow> p = 0"
   apply (simp add: canonical_address_def canonical_address_of_def level_defs pt_bits_left_def
                    bit_simps is_aligned_nth)
-  apply word_bitwise
-  apply clarsimp
-  done
+  by word_bitwise clarsimp
 
 lemma aligned_vref_for_level[simp]:
   "is_aligned (vref_for_level vref level) (pt_bits_left level)"
@@ -1911,7 +1933,7 @@ lemma user_region_slots:
   apply (clarsimp simp: valid_uses_user_region_eq kernel_mapping_slots_def pt_index_def level_defs)
   apply (simp add: pt_bits_left_def bit_simps canonical_address_def canonical_address_of_def)
   apply word_bitwise
-  by (clarsimp simp: word_bits_def canonical_bit_def word_size)
+  by (clarsimp simp: word_bits_def canonical_bit_def word_size user_vtop_def pptrUserTop_def)
 
 lemma valid_vspace_objs_strongD:
   "\<lbrakk> valid_vspace_objs s;
