proof/invariant-abstract/RISCV64/ArchKernelInit_AI.thy
@@ -21,6 +21,18 @@ text {*
   Showing that there is a state that satisfies the abstract invariants.
 *}
 
+definition
+  "init_vspace_uses p \<equiv>
+     if p \<in> {pptr_base ..< kernel_base} then RISCVVSpaceKernelWindow
+     else if kernel_base \<le> p then RISCVVSpaceKernelELFWindow
+     else if p \<le> user_vtop then RISCVVSpaceUserRegion
+     else RISCVVSpaceInvalidRegion"
+
+lemma "valid_uses_2 init_vspace_uses"
+  using user_vtop_pptr_base pptr_base_kernel_base user_vtop_pptr_base[simp del]
+  unfolding valid_uses_2_def init_vspace_uses_def
+  by (auto intro: below_user_vtop_canonical above_pptr_base_canonical)
+
 (* FIXME RISCV: TODO *)
 
 end
